Bytestring example ready

examples/bytestring/main.c
@@ -3,7 +3,6 @@
 #include "gc.h"
 
 extern value body(struct thread_info *);
-extern void print_Coq_Init_Datatypes_nat(int_or_ptr64);
 
 _Bool is_ptr(unsigned int s) {
   return (_Bool) Is_block(s);
@@ -15,6 +14,5 @@ int main(int argc, char *argv[]) {
   tinfo = make_tinfo();
   body(tinfo);
 
-  puts("");
   return 0;
 }
