examples/bytestring/prims.c
@@ -2,6 +2,7 @@
 #include "glue.h"
 #include <stddef.h>
 #include <stdio.h>
+#include <string.h>
 
 #define LIVEPOINTERS0(tinfo, exp) (exp)
 #define LIVEPOINTERS1(tinfo, exp, a) ({ \
@@ -53,73 +54,308 @@
   a = __ROOT__[0]; b = __ROOT__[1]; c = __ROOT__[2]; d = __ROOT__[3]; e = __ROOT__[4]; f = __ROOT__[5]; g = __ROOT__[6]; h = __ROOT__[7]; \
   tinfo->fp = __FRAME__.prev; __TEMP__; })
 
-typedef enum { O, S } nat;
-unsigned long long nat_to_ull(value n) {
-  value temp = n;
-  unsigned int i = 0;
-
-  while(1) {
-    unsigned int tag = get_Coq_Init_Datatypes_nat_tag(temp);
-    if(tag == S) {
-      i++;
-      temp = get_Coq_Init_Datatypes_S_args(temp)->Coq_Init_Datatypes_S_arg_0;
-    } else {
-      break;
-    }
-  } 
-  return i;
+value bytestrlen(value s)
+{
+  value *ptr = (value *) s;
+  value *headerptr = ptr - 1;
+  value header = *headerptr;
+  value words = header >> 10;
+  value bytes = words * sizeof(value);
+  value padding = (value) *((char *) s + (bytes - 1)) + 1;
+  return bytes - padding;
 }
 
-typedef enum { PURE, BIND, SET, GET } mi;
-value runM(struct thread_info *tinfo, unsigned long long size, value init, value arr, value action) {
-  value i, temp, arg0, arg1;
-  switch (get_prog_C_MI_tag(action)) {
-    case PURE:
-      return get_prog_C_pureI_args(action)->prog_C_pureI_arg_1;
-    case BIND:
-      arg0 = get_prog_C_bindI_args(action)->prog_C_bindI_arg_2;
-      arg1 = get_prog_C_bindI_args(action)->prog_C_bindI_arg_3;
-      temp = LIVEPOINTERS4(tinfo, runM(tinfo, size, init, arr, arg0), arg0, arg1, init, arr);
-      temp = LIVEPOINTERS4(tinfo, call(tinfo, arg1, temp), arg1, init, arr, temp);
-      return runM(tinfo, size, init, arr, temp);
-    case SET:
-      arg0 = get_prog_C_setI_args(action)->prog_C_setI_arg_0;
-      i = nat_to_ull(arg0);
-      arg1 = get_prog_C_setI_args(action)->prog_C_setI_arg_1;
-      // check if there's enough memory for the update record (1 word)
-      if (!(1 <= tinfo->limit - tinfo->alloc)) {
-        tinfo->nalloc = 1;
-        LIVEPOINTERS2(tinfo, garbage_collect(tinfo), arr, arg1);
-      }
-      if (i < size) {
-        certicoq_modify(tinfo, (value *) arr + i, arg1);
-      }
-      return make_Coq_Init_Datatypes_unit_tt();
-    case GET:
-      arg0 = get_prog_C_getI_args(action)->prog_C_getI_arg_0;
-      i = nat_to_ull(arg0);
-      if (i < size) {
-        return *((value *) arr + i);
-      } else {
-        return init;
-      }
+/* value bytestrlen(value s) */
+/* { */
+/*   value words = (*((value *) s - 1) >> 10); */
+/*   value bytes = words * sizeof(value); */
+/*   value padding = (value) *((char *) s + (bytes - 1)) + 1; */
+/*   return bytes - padding; */
+/* } */
+
+unsigned char ascii_to_char(value x) {
+  unsigned char c = 0;
+  for(unsigned int i = 0; i < 8; i++) {
+    unsigned int tag = get_Coq_Init_Datatypes_bool_tag(*((value *) *((value *) x) + i));
+    c += !tag << i;
   }
+  return c;
 }
 
-value array_runM(struct thread_info *tinfo, value a, value len, value init, value action) {
-  size_t size = nat_to_ull(len);
-  size_t nalloc = size + 1;
-  // check if there's enough memory for the array (size + 1 word for header)
+/////////////////////////////////////////////////////////////////
+
+value bool_to_value(_Bool b) {
+  if(b)
+    return make_Coq_Init_Datatypes_bool_true();
+  else
+    return make_Coq_Init_Datatypes_bool_false();
+}
+
+value char_to_value(struct thread_info *tinfo, char c) {
+  value v[8];
+  for(unsigned int i = 0; i < 8; i++) {
+    v[i] = bool_to_value(c & (1 << i));
+  }
+  return alloc_make_Coq_Strings_Ascii_ascii_Ascii(tinfo, v[0], v[1], v[2], v[3], v[4], v[5], v[6], v[7]);
+}
+
+value string_to_value(struct thread_info *tinfo, char *s) {
+  value temp = make_Coq_Strings_String_string_EmptyString();
+  for (unsigned int i = strlen(s); 0 < i; i--) {
+    value c = char_to_value(tinfo, s[i-1]);
+    temp = alloc_make_Coq_Strings_String_string_String(tinfo, c, temp);
+  }
+  return temp;
+}
+
+/////////////////////////////////////////////////////////////////
+
+/*
+value word8_to_ascii(struct thread_info *tinfo, value w)
+{
+  fprintf(stderr, "word8_to_ascii unimplemented");
+  exit(EXIT_FAILURE);
+}
+value ascii_to_word8(struct thread_info *tinfo, value v)
+{
+  fprintf(stderr, "ascii_to_word8 unimplemented");
+  exit(EXIT_FAILURE);
+}
+
+value to_upper(struct thread_info *tinfo, value v)
+{
+  char c = (char) (v >> 1); 
+  char up = toupper(c);
+  return (((value) up) << 1) + 1;
+}
+
+value map(struct thread_info *tinfo, value f, value s)
+{
+  value len = bytestrlen(s);
+
+  value mod = len % sizeof(value);
+  value pad_length = sizeof(value) - (len % sizeof(value));
+  value needed = (len + pad_length) / sizeof(value) + 1;
+  if (!(needed <= tinfo->limit - tinfo->alloc)) {
+    fprintf(stderr, "not enough memory, call GC");
+    exit(EXIT_FAILURE);
+  }
+
+  value *argv = (value *) tinfo->alloc;
+  *((value *) argv + 0LLU) = ((needed - 1) << 10) + 252LLU; // string tag
+
+  char *ptr = (char *) (argv + 1LLU);
+  char *t = (char *) s;
+  for (value i = 0; i < len; i++) {
+    value c = (*t << 1) + 1;
+    *ptr = call(tinfo, f, c) >> 1;; 
+    ptr++; t++; 
+  }
+
+  // make the padding
+  char i = 0;
+  while (i < pad_length - 1) { *ptr = 0; ptr++; i++; }
+  *ptr = i; // last char in the padding is # of 0s coming before the last char
+
+  tinfo->alloc += needed;
+  return (value) (argv + 1LLU);
+}
+*/
+
+value append(struct thread_info *tinfo, value s1, value s2)
+{
+  value len1 = bytestrlen(s1);
+  value len2 = bytestrlen(s2);
+  value sum = len1 + len2;
+  value mod = sum % sizeof(value);
+  value pad_length = sizeof(value) - (sum % sizeof(value));
+  value nalloc = (sum + pad_length) / sizeof(value) + 1;
   if (!(nalloc <= tinfo->limit - tinfo->alloc)) {
     tinfo->nalloc = nalloc;
-    LIVEPOINTERS2(tinfo, garbage_collect(tinfo), init, action);
+    LIVEPOINTERS2(tinfo, garbage_collect(tinfo), s1, s2);
   }
-  value *arr = tinfo->alloc;
-  arr[0LLU] = size << 10;
-  arr = arr + 1LLU;
-  for (size_t i = 0; i < size; i++) {
-    arr[i] = init;
-  }
+
+  value *argv = (value *) tinfo->alloc;
+  *((value *) argv + 0LLU) = ((nalloc - 1) << 10) + 252LLU; // string tag
+  
+  // take a pointer pointing to the beginning of destination string
+  char *ptr = (char *) (argv + 1LLU);
+  char *t1 = (char *) s1;
+  char *t2 = (char *) s2;
+
+  // copy the OCaml-string pointed by t1 and t2
+  // into the array pointed by ptr
+  // skip the padding in each one, we'll make our own padding later
+  for (value i = 0; i < len1; i++) { *ptr = *t1; ptr++; t1++; }
+  for (value i = 0; i < len2; i++) { *ptr = *t2; ptr++; t2++; }
+
+  // make the padding
+  char i = 0;
+  while (i < pad_length - 1) { *ptr = 0; ptr++; i++; }
+  *ptr = i; // last char in the padding is # of 0s coming before the last char
+
   tinfo->alloc += nalloc;
-  return runM(tinfo, size, init, (value) arr, action);
+  return (value) (argv + 1LLU);
+}
+
+value pack(struct thread_info *tinfo, value s)
+{
+  value temp = s;
+  value len = 0;
+  while(get_Coq_Strings_String_string_tag(temp) == 1) {
+    len++;
+    temp = *((value *) temp + 1ULL);
+  } 
+  value mod = len % sizeof(value);
+  value pad_length = sizeof(value) - (len % sizeof(value));
+  value nalloc = (len + pad_length) / sizeof(value) + 1;
+  if (!(nalloc <= tinfo->limit - tinfo->alloc)) {
+    tinfo->nalloc = nalloc;
+    LIVEPOINTERS1(tinfo, garbage_collect(tinfo), s);
+  }
+
+  value *argv = (value *) tinfo->alloc;
+  *((value *) argv + 0LLU) = ((nalloc - 1) << 10) + 252LLU; // string tag
+
+  char *ptr = (char *) (argv + 1LLU);
+  temp = s;
+  while(get_Coq_Strings_String_string_tag(temp) == 1) {
+    *ptr = ascii_to_char(temp);
+    ptr++;
+    temp = *((value *) temp + 1ULL);
+  } 
+
+  // make the padding
+  char i = 0;
+  while (i < pad_length - 1) { *ptr = 0; ptr++; i++; }
+  *ptr = i; // last char in the padding is # of 0s coming before the last char
+
+  tinfo->alloc += nalloc;
+  return (value) (argv + 1LLU);
+}
+
+
+value unpack(struct thread_info *tinfo, value bs)
+{
+  // 3 for the String constructor, 9 for the ASCII constructor.
+  value nalloc = bytestrlen(bs) * (3 + 9);
+  if (!(nalloc <= tinfo->limit - tinfo->alloc)) {
+    tinfo->nalloc = nalloc;
+    LIVEPOINTERS1(tinfo, garbage_collect(tinfo), bs);
+  }
+
+  char *s = (char *) bs;
+  value temp = make_Coq_Strings_String_string_EmptyString();
+  for (unsigned int i = bytestrlen(bs); 0 < i; i--) {
+    value c = char_to_value(tinfo, s[i-1]);
+    temp = alloc_make_Coq_Strings_String_string_String(tinfo, c, temp);
+  }
+  return temp;
+}
+
+// from https://codereview.stackexchange.com/a/207541/68819
+// allocates enough memory for a string (which has to be freed later)
+// returns its length by assigning it to the pointer in the argument
+char *scan(FILE *stream, size_t *length)
+{
+  size_t capacity = 16;
+  char *buffer = malloc(capacity);
+  if (!buffer) { return NULL; }
+  size_t i = 0;
+
+  int c; // current input character
+  while ((c = fgetc(stream)) != EOF) {
+    if (i + 2 > capacity) {
+      // ensure space for c and terminating NUL
+      capacity *= 2;
+      char *newbuf = realloc(buffer, capacity);
+      if (!newbuf) {
+        // allocation failed - undo the read, terminate string, and return
+        ungetc(c, stdin);
+        buffer[i] = '\0';
+        return buffer;
+      }
+      buffer = newbuf;
+    }
+
+    // We have enough space; now store it
+    if (c == '\n') { break; }
+    buffer[i++] = (char) c;
+  }
+
+  if (i == 0) { free(buffer); return NULL; } // we didn't read anything
+
+  buffer[i] = '\0';
+  *length = i;
+
+  return buffer;
+}
+
+value scan_bytestring(struct thread_info *tinfo, value instream)
+{
+  size_t len;
+  char *s = scan((FILE *) instream, &len);
+
+  value mod = len % sizeof(value);
+  value pad_length = sizeof(value) - (len % sizeof(value));
+  value nalloc = (len + pad_length) / sizeof(value) + 1;
+  if (!(nalloc <= tinfo->limit - tinfo->alloc)) {
+    tinfo->nalloc = nalloc;
+    LIVEPOINTERS1(tinfo, garbage_collect(tinfo), instream);
+  }
+
+  value *argv = (value *) tinfo->alloc;
+  *((value *) argv + 0LLU) = ((nalloc - 1) << 10) + 252LLU; // string tag
+
+  char *ptr = (char *) (argv + 1LLU);
+  char *t = (char *) s;
+  while (*t != '\0') { *ptr = *t; ptr++; t++; }
+
+  // make the padding
+  char i = 0;
+  while (i < pad_length - 1) { *ptr = 0; ptr++; i++; }
+  *ptr = i; // last char in the padding is # of 0s coming before the last char
+
+  tinfo->alloc += nalloc;
+  return (value) (argv + 1LLU);
+}
+
+/////////////////////////////////////////////////////////////////
+
+typedef enum { PURE, BIND, PRINT, SCAN } M;
+value runM(struct thread_info * tinfo, value a, value instream, value outstream, value action)
+{
+  value temp, arg0, arg1;
+  switch (get_prog_C_MI_tag(action)) {
+    case PURE:
+      return get_args(action)[1];
+    case BIND:
+      arg0 = get_args(action)[2];
+      arg1 = get_args(action)[3];
+      temp = LIVEPOINTERS4(tinfo, runM(tinfo, a, instream, outstream, arg0), arg0, arg1, instream, outstream);
+      temp = LIVEPOINTERS4(tinfo, call(tinfo, arg1, temp), arg1, instream, outstream, temp);
+      return runM(tinfo, a, instream, outstream, temp);
+    case PRINT:
+      {
+        value s = *((value *) action);
+        value len = bytestrlen(s);
+        for (value i = 0; i < len; i ++) {
+          fprintf((FILE *) outstream, "%c", ((char *) s)[i]);
+        }
+        fprintf((FILE *) outstream, "\n");
+        return 0;
+      }
+    case SCAN:
+      return scan_bytestring(tinfo, instream);
+    default:
+      return 0;
+  }
+}
+
+value get_stdin(struct thread_info * tinfo, value _tt) {
+  return stdin;
+}
+
+value get_stdout(struct thread_info * tinfo, value _tt) {
+  return stdout;
 }
