examples/bytestring/prims.h
@@ -1,3 +1,6 @@
-value nat_to_ull(value);
-value runM(struct thread_info *tinfo, value, value);
-value array_runM(struct thread_info *tinfo, value, value, value, value);
+value append(struct thread_info *tinfo, value, value);
+value pack(struct thread_info *tinfo, value);
+value unpack(struct thread_info *tinfo, value);
+value runM(struct thread_info *tinfo, value, value, value, value);
+value get_stdin(struct thread_info *tinfo, value);
+value get_stdout(struct thread_info *tinfo, value);
