examples/bytestring/Verif_prog.v
@@ -1,0 +1,17 @@
+Require Import ZArith.
+Require Import Psatz.
+
+Require Import VeriFFI.generator.funspec.
+Require Import VeriFFI.generator.Rep.
+
+(* Obligation Tactic := gen. *)
+(* MetaCoq Run (gen_for nat). *)
+(* MetaCoq Run (gen_for unit). *)
+
+Require Import VeriFFI.examples.bytestring.prog.
+Require Import VeriFFI.examples.bytestring.model.
+
+Import Bytestring_Proofs.
+Check pure_desc.
+
+Check (fn_desc_to_funspec pure_desc).
