generator/funspec.v
@@ -43,51 +43,27 @@ Fixpoint in_graphs
   | RES x _ => fun _ => ps = nil
   end xs.
 
-Definition ep_to_funspec_aux
+Definition fn_desc_to_funspec_aux
            (c : reified prim_ann)
            (uncurried_model_fn : meta.reflect c)
            (arity : nat) : funspec :=
-  NDmk_funspec
-    (get_c_typesig c arity)
-    cc_default
-    (globals * graph * GCGraph.roots_t * share * args c * list rep_type *
-       val * GCGraph.outlier_t * GCGraph.fun_info * GCGraph.thread_info)
-    (fun x => match x with
-     | (gv, g, roots, sh, xs, ps, ti, outlier, f_info, t_info) =>
+  WITH gv : globals, g : graph, roots : GCGraph.roots_t, sh : share,
+       xs : args c, ps : list rep_type, ti : val,
+       outlier : GCGraph.outlier_t, f_info : GCGraph.fun_info, t_info : GCGraph.thread_info
+   PRE [[ cons t_tinfo (repeat tvalue arity) ]]
        PROP (writable_share sh ;
               in_graphs g c xs ps)
        (PARAMSx (ti :: map (rep_type_val g) ps)
-       (SEPx (full_gc g t_info roots outlier ti sh :: nil)))
-     end)
-    (fun x => match x with
-     | (gv, g, roots, sh, xs, ps, ti, outlier, f_info, t_info) =>
+         (SEPx (full_gc g t_info roots outlier ti sh :: nil)))
+   POST [ tvalue ]
        EX (p' : rep_type) (g' : graph) (t_info' : GCGraph.thread_info),
           PROP (let r := result c xs in
                 @is_in_graph (projT1 r) (@prim_in_graph (projT1 r) (projT2 r)) g'
                   (uncurried_model_fn xs) p' ;
                 gc_graph_iso g roots g' roots)
           RETURN  (rep_type_val g' p')
-          SEP (full_gc g' t_info' roots outlier ti sh)
-     end).
+          SEP (full_gc g' t_info' roots outlier ti sh).
 
-Definition ep_to_funspec (d : fn_desc) (xs : args (type_desc d)) : ident * funspec :=
+Definition fn_desc_to_funspec (d : fn_desc) (xs : args (type_desc d)) : ident * funspec :=
   (ident_of_string (c_name d),
-   ep_to_funspec_aux (type_desc d) (uncurried_model_fn d) (f_arity d)).
-
-(* Definition uint63_to_nat_spec :  funspec :=  *)
-(*    WITH gv : globals, g : graph, roots : roots_t, sh : share, n: nat, *)
-(*         ti : val, outlier : outlier_t, f_info : fun_info, t_info : GCGraph.thread_info *)
-(*    PRE  [ tptr t_tinfo,  (talignas 3%N (tptr tvoid)) ] *)
-(*       PROP ( (Z.of_nat n) < headroom t_info ; (* KS: 2 times this *) *)
-(*             writable_share sh  *)
-(*             (* min_signed <= encode_Z (Z.of_nat n) <= max_signed *) *)
-(*             ) *)
-(*       (PARAMSx [ti; Vlong (Int64.repr (encode_Z (Z.of_nat n)))] *)
-(*       (GLOBALSx nil *)
-(*       (SEPx (full_gc g t_info roots outlier ti sh :: nil)))) *)
-(*    POST [ (talignas 3%N (tptr tvoid)) ] *)
-(*      EX (p' : rep_type) (g' : graph) (t_info' : GCGraph.thread_info), *)
-(*        PROP (@is_in_graph nat (@in_graph nat _) g' n p' ; *)
-(*              gc_graph_iso g roots g' roots) *)
-(*        RETURN  (rep_type_val g' p') *)
-(*        SEP (full_gc g' t_info' roots outlier ti sh) . *)
+   fn_desc_to_funspec_aux (type_desc d) (uncurried_model_fn d) (f_arity d)).
